\documentclass[10pt,twocolumn]{article}
\usepackage[margin=0.5in]{geometry}
\usepackage[cmex10]{amsmath}
\usepackage{amsmath}
\usepackage{amsmath,amssymb,amsfonts}
\usepackage{graphicx}
\usepackage{textcomp}
\usepackage{amsmath,amssymb,amsfonts,amsthm}
\usepackage{gensymb}
\usepackage{mathtools}
\newcommand*{\Comb}[2]{{}^{#1}C_{#2}}%
\title{
Probability Assignment
}
\author{GINNA SHREYANI}
\date{}
\begin{document}
\maketitle


\textbf{12.13.1.5}\\
If P(A)=$\frac{6}{11}$, $P(B)=\frac{5}{11}$ and P(A+B)=$\frac{7}{11}$, find\\
(i) P(A.B)   (ii)P($A \mid B$)  (iii)P($B\mid A$)
\subsection*{Solution}
\textbf{(i)} We know that,\\
\begin{equation}
	P(A.B) = P(A) + P(B) -P(A+B)
	\label{eq-1}
\end{equation}
From ($\ref{eq-1}$), we get\\
\begin{align*}
	&P(A.B) = \frac{6}{11} + \frac{5}{11} - \frac{7}{11}\\
	&P(A.B) = \frac{4}{11}
\end{align*}
\textbf{(ii)}, We know that,\\
\begin{equation}
	P(A\mid B) = \frac{P(A.B)}{P(B)}
	\label{eq-2}
\end{equation}
From ($\ref{eq-2}$), we get\\
\begin{align*}
	&P(A \mid B) = \frac{\frac{4}{11}}{\frac{5}{11}}\\
	&P(A\mid B) = \frac{4}{5}
\end{align*}
\textbf{(iii)}, We know that,\\
\begin{equation}
	P(B\mid A)=\frac{P(B.A)}{P(A)}
	\label{eq-3}
\end{equation}
From ($\ref{eq-3}$), we get\\
\begin{align*}
	&P(B\mid A) = \frac{\frac{4}{11}}{\frac{6}{11}}\\
	&P(B\mid A) = \frac{4}{6}\\
	&P(B\mid A) = \frac{2}{3}
\end{align*}
As a result,
\begin{align*}
	&P(A.B) = \frac{4}{11}\\
	&P(A\mid B) = \frac{4}{5}\\
	&P(B\mid A) = \frac{2}{3}
\end{align*}
\end{document}
